

Extended euclid

$$ax_0 + by_0 = d$$

$$\Leftrightarrow bx_1 + [a - b \cdot \text{int}(\frac{a}{b})]y_1 = d$$

$$\Leftrightarrow bx_1 + ay_1 - b \cdot \text{int}(\frac{a}{b})y_1 = d$$

$$\Leftrightarrow ay_1 + b(x_1 - \text{int}(\frac{a}{b})y_1) = d$$

$$\rightarrow \begin{cases} x_0 = y_1 \\ y_0 = x_1 - y_1 \cdot \text{int}(\frac{a}{b}) \end{cases}$$

Nghiệm Diophantine

Từ bđt Bezout, ta có:

$$(a, b) \Leftrightarrow ax + by = d = (a, b)$$

$$\text{Nếu } d \mid c \text{ thì } c = d \cdot k \Leftrightarrow k = \frac{c}{d}$$

$$\text{Ta có } \Leftrightarrow ax \cdot \frac{c}{d} + by \cdot \frac{c}{d} = c$$

$$\rightarrow \begin{cases} x_0 = x \cdot \frac{c}{d} \\ y_0 = y \cdot \frac{c}{d} \end{cases} \rightarrow \text{Dùng Extended euclid để tìm } (x; y)$$

Nghiệm tổng quát diophantine

$$\text{Xét } ax + by = c, \text{ gọi } d = (a, b)$$

$$\Leftrightarrow a(x_0 + \frac{b}{d}) + b(y_0 - \frac{a}{d}) = c$$

$$\text{Kiểm tra: } ax_0 + by_0 + \frac{ab}{d} - \frac{ab}{d} = c \text{ (thỏa)}$$

$$\rightarrow \begin{cases} x = x_0 + k \cdot \frac{b}{d} \\ y = y_0 - k \cdot \frac{a}{d} \end{cases} \quad (k \in \mathbb{Z})$$

* Nghiệm nguyên dương $(x, y > 0)$

$$\Leftrightarrow \begin{cases} x_0 + k \frac{b}{d} > 0 \\ y_0 - k \frac{a}{d} > 0 \end{cases} \Leftrightarrow \begin{cases} k > -x_0 \cdot \frac{d}{b} \\ k < y_0 \cdot \frac{d}{a} \end{cases} \rightarrow -x_0 \cdot \frac{d}{b} < k < y_0 \cdot \frac{d}{a}$$